ftlr: retrieve

theories/logrel/logrel.v
@@ -14,8 +14,10 @@ Section logrel.
   Definition pages_in_trans (trans: gmap Word transaction) : gset PID :=
     map_fold (λ (k:Addr) v acc, v.1.1.2 ∪ acc) (∅: gset PID) trans.
 
+  Definition trans_ps_disj trans := map_Forall (λ h tran, tran.1.1.2 ## pages_in_trans (delete h trans)) trans.
+
   Definition pgt (ps: gset PID) q (vo: VMID) (be: bool) : iProp Σ :=
-    [∗ set] p ∈ ps, p -@{q}O> vo ∗ p -@{q}E> be.
+    ([∗ set] p ∈ ps, p -@{q}O> vo) ∗ [∗ set] p ∈ ps, p -@{q}E> be.
 
   (** definitions **)
 
@@ -28,32 +30,28 @@ Section logrel.
   (* [pagetable_entries_excl_owned]: For pages that are exclusively accessible and owned by i, i keeps the entries. *)
   Definition pagetable_entries_excl_owned (i:VMID) (ps: gset PID) := pgt ps 1 i true.
 
-
-
   (* [transaction_hpool_global_transferred]: All of half of transactions, as we don't know which one would be used by i. *)
   (* We need the pure proposition to ensure all transaction entries are transferred.
-     Only half is needed so that the invokers can remember transactions by keeping the other half.
-     Holding half of pagetable entries gives us extra properties... [TODO] *)
+     Only half is needed so that the invokers can remember transactions by keeping the other half.*)
   Definition transaction_hpool_global_transferred (trans: gmap Addr transaction) : iProp Σ:=
-    ∃ hpool,  ⌜hpool ∪ dom (gset _ ) trans = hs_all⌝ ∗ fresh_handles 1 hpool ∗
-    [∗ map] h ↦ tran ∈ trans, h -{1/2}>t tran.1 ∗ pgt tran.1.1.2 (1/2)%Qp tran.1.1.1.1.1 (bool_decide (tran.1.2 ≠ Sharing)).
+    ∃ hpool,  ⌜hpool ∪ dom (gset _ ) trans = hs_all⌝ ∗ fresh_handles 1 hpool ∗ ⌜trans_ps_disj trans⌝ ∗ [∗ map] h ↦ tran ∈ trans, h -{1/2}>t tran.1.
 
   (* [transaction_pagetable_entries_owned]: transaction and page table entries that are owned initially by i,
      i.e. they are not transferred by VMProp, so we doesn't need to take care of them when reasoning the primary VM.
      As the invoker of sharing and lending transactions, i always has the ownership of involved pages.
-     Therefore, i ownes half of these pagetable entries even if they are in some transactions.
+     Therefore, i ownes these pagetable entries even if they are in some transactions.
      Furthermore, since it is suffice for the receiver to retrieve or relinquish with half of transacitons entries,
      while the sender needs full to reclaim, we let i always own half and only pass the otner half around with VMProp*)
   (* [TODO] relation to [pagetable_entries_excl_owned] *)
   Definition transaction_pagetable_entries_owned (trans: gmap Addr transaction) : iProp Σ:=
-    big_sepFM trans (λ kv, kv.2.1.1.1.1.1 = i ∧ kv.2.1.2 ≠ Donation) (λ k v, k -{1/2}>t v.1 ∗ pgt v.1.1.2 (1/2)%Qp v.1.1.1.1.1 (bool_decide (v.1.2 ≠ Sharing)))%I.
+    big_sepFM trans (λ kv, kv.2.1.1.1.1.1 = i ∧ kv.2.1.2 ≠ Donation) (λ k v, k -{1/2}>t v.1 ∗ pgt v.1.1.2 1 v.1.1.1.1.1 (bool_decide (v.1.2 ≠ Sharing)))%I.
 
    (* [transaction_pagetable_entries_transferred] : For donation, the half of transaction entries that are kept by sender in case
       of sharing and lending are also be passed around between the sender and the receiver, as retrieval in this case also requires
       full entries.
       Pagetable entries are transferred along as both sender and receiver could be the exclusive owner of those pages. *)
   Definition transaction_pagetable_entries_transferred (trans: gmap Addr transaction) : iProp Σ:=
-    big_sepFM trans (λ kv, kv.2.1.2 = Donation ∧ (kv.2.1.1.1.2 = i ∨ kv.2.1.1.1.1.1 = i)) (λ k v, k -{1/2}>t v.1 ∗ pgt v.1.1.2 (1/2)%Qp v.1.1.1.1.1 true)%I.
+    big_sepFM trans (λ kv, kv.2.1.2 = Donation ∧ (kv.2.1.1.1.2 = i ∨ kv.2.1.1.1.1.1 = i)) (λ k v, k -{1/2}>t v.1 ∗ pgt v.1.1.2 1 v.1.1.1.1.1 true)%I.
 
   (* [retrieval entries]: half of all retrieval entries of i-related transactions are required.
      For transactions where i is the sender, we need the corresponding retrieval entries to check if it is allowed for i to reclaim,
@@ -73,16 +71,16 @@ Section logrel.
 
   Definition VMProp_unknown p_tx p_rx trans : iProp Σ:=
     ∃ ps_na' ps_acc' (trans' : gmap Word transaction) rx_state ,
-               let ps_oea := ps_acc' ∖ {[p_rx;p_tx]} ∖ pages_in_trans (trans_memory_in_trans trans) in
-               let ps_macc_trans' := pages_in_trans (trans_memory_in_trans trans') in
-               let ps_oea' := ps_acc' ∖ {[p_rx;p_tx]} ∖ ps_macc_trans' in
+               let ps_oea := ps_acc' ∖ {[p_rx;p_tx]} ∖ (pages_in_trans trans)  in
+               let ps_macc_trans' := (pages_in_trans (trans_memory_in_trans trans')) in
+               let ps_oea' := ps_acc' ∖ {[p_rx;p_tx]} ∖ pages_in_trans trans' in
                (* lower bound *)
                i -@{1/2}A> ps_acc' ∗
                LB@ i := [ps_na'] ∗
                (* NOTE: Just having [ps_acc'] seems not enough, which can be broken by getting access to pages in ps_na from some
                 transaction. *)
                (* XXX: how to formulate the disjointness using RAs? making use of ownership and exclusiveness? *)
-               ⌜ps_na' ## (ps_acc' ∪ ps_macc_trans')⌝ ∗
+               ⌜ps_na' ## ps_acc' ∪ ps_macc_trans'⌝ ∗
                (* we can derive ⌜{[p_rx;p_tx]} ## ps_mem_in_trans''⌝ from rx_page/tx_page ∗ transaction_hpool_global_transferred *)
                (* transaction and pagetable entries *)
                transaction_hpool_global_transferred trans' ∗
@@ -134,9 +132,9 @@ Section logrel.
 
   Program Definition interp_access p_tx p_rx ps_acc trans : iPropO Σ:=
     (
-      let ps_mem_in_trans := pages_in_trans (trans_memory_in_trans trans) in
+      (* let ps_mem_in_trans := pages_in_trans (trans_memory_in_trans trans) in *)
       (* exclusively owned pages are pages i has access to, but ain't in any transactions related to i. *)
-      let ps_oea := ps_acc ∖ {[p_rx;p_tx]} ∖ ps_mem_in_trans in
+      let ps_oea := ps_acc ∖ {[p_rx;p_tx]} ∖ (pages_in_trans trans) in
       (* registers *)
       (∃ regs, ⌜is_total_gmap regs⌝ ∗ [∗ map] r ↦ w ∈ regs, r @@ i ->r w) ∗
       (* TX page and its memory *)
